\noindent A grammar is LL(1) if and only if, for all rules 
\begin{center}
    $A \rightarrow \beta | \gamma $ 
    
    $la(A \rightarrow \beta) \cap la(A \rightarrow \gamma) = \varnothing$
\end{center}
with $(\beta \ne \gamma)$  \\

\noindent It is not LL(1) as:
\begin{center}
    $first_{1}(S \rightarrow ab) = first_{1}(S \rightarrow ac) = \{a\}$
\end{center}

\noindent It is LL(2) as:
\begin{center}
    $first_{2}(S \rightarrow ab) = \{ab\} \ne first_{2}(S \rightarrow ac) = \{ac\}$
\end{center}